case_studies/illc/fllc_ext.v
@@ -4,8 +4,7 @@
 
 (* Imports *)
 From Coq Require Import Lia Logic.FunctionalExtensionality
-                        Program.Equality Logic.JMeq
-                        Unicode.Utf8.
+                        Program.Equality Logic.JMeq Unicode.Utf8.
 From Hammer Require Import Hammer.
 From VST.msl Require Import sepalg functors.
 From CARVe Require Import contexts.total_fun algebras.dill.
